src/Utils.dfy
@@ -145,4 +145,6 @@ module Seq {
   {
     xs[..i] + xs[i+1..]
   }
+
+
 }
